\documentclass[xcolor=table]{beamer}
\usetheme{Dresden} % My favorite!
\usecolortheme{beaver} % Simple and clean template
\usepackage{amssymb,latexsym}
\usepackage{xltxtra, xgreek}
\usepackage{graphicx}
\usepackage{textcomp}
\usepackage{url} 

\setsansfont[Mapping=tex-text]{CMU Concrete}
\setmonofont{Courier New}
\newcommand{\tab}{\hspace*{1.2em}}

\definecolor{links}{HTML}{E4287C}
\hypersetup{colorlinks,linkcolor=,urlcolor=links}
\definecolor{gray}{gray}{0.89}

%\usetheme{Boadilla} % Pretty neat, soft color.
%\usetheme{default}
%\usetheme{Warsaw}
%\usetheme{Bergen} % This template has nagivation on the left
%\usetheme{Frankfurt} % Similar to the default 
%with an extra region at the top.
%\usecolortheme{seahorse} % Simple and clean template
%\usetheme{Darmstadt} % not so good
% Uncomment the following line if you want %
% page numbers and using Warsaw theme%
% \setbeamertemplate{footline}[page number]
\setbeamercovered{transparent}
%\setbeamercovered{invisible}
% To remove the navigation symbols from 
% the bottom of slides%
\setbeamertemplate{navigation symbols}{} 
\expandafter\def\expandafter\insertshorttitle\expandafter{%
  \insertshorttitle\hfill\insertframenumber\,/\,\inserttotalframenumber}
  

 
\newcommand{\bs}[1]{\boldsymbol{#1}}  
\renewcommand{\figurename}{Figure \arabic{figure}}

%\usepackage{bm}         % For typesetting bold math (not \mathbold)
%\logo{\includegraphics[height=0.6cm]{yourlogo.eps}}
%
\title[The Jebus Lambda Calculus Interpreter]{Υλοποίηση ενός διερμηνέα για Λάμβδα Λογισμό}
\author{Ζωή Παρασκευοπούλου \\ \and Νίκος Γιανναράκης  }

\institute[]
{
Σχολή Ηλεκτρολόγων Μηχανικών και Μηχανικών Υπολογιστών\\
Εθνικό Μετσόβιο Πολυτεχνείο
}
\date{\today}
\begin{document}

\begin{frame}
\titlepage
\end{frame}

%% Dependencies
% wl-pprint
% parsec
% cmdargs

\begin{frame}
\frametitle{The Syntax}
\begin{block}
{
\begin{small}
\begin{align*}
e & := e_1 \; e_2 																		                                  & op &:= \bs{``+"}\; | \; \bs{``-"}  \\
   & | \; \bs{``\lambda"} \; id \; \bs{`` ."} \; e 										                  &        & |\; \bs{``*"} \; 	  \\
   & | \; \bs{``let"} \; [\bs{``rec"}] \; id \; \bs{``="} \; e_1 \; \bs{``in"} \; e_2 		  & 		& | \; \bs{``**"}		              \\
   & | \;  \bs{``["}e1\bs{``,"} \; e2\bs{``]"} 													              & rop & := \bs{``="} | \bs{``<"}\\
   & | \;  id 																			 	                                  & 		& | \bs{``<="} | \bs{``>"}\\
   & | \;  \bs{``true"}\; | \;\bs{``false"} 													                  &		& | \bs{``>="} \\
   & | \; \bs{``if"}\; \; e_1\; \bs{``then"}\; e_2\; \bs{``else"}\; e_3    & bop & := \bs{``\&\&"} \\
   & | \; e_1 \; op \; e_2                                                                                         &             & | \bs{``||"} \\
   & | \; e_1 \; rop \; e_2                                                                                          & \\
   & | \; e_1 \; bop \; e_2
\end{align*}
\end{small}

}

\end{block}
\end{frame}

%


\begin{frame}
\frametitle{Type System}
\begin{block}
{
The language is strongly typed featuring the \textbf{Hindley-Milner} type system. The types are implicit in the source (à la Curry) and they are automatically reconstructed using the \textbf{algorithm W} for type inference.
}
\end{block}


\end{frame}


\begin{frame}
\frametitle{Hindley-Milner typing}
\begin{block}
{ 
Hindley-Milner type system is a restriction of system F, featuring let polymorphism. Unlike system F, in which type reconstruction is undecidable, 
the types can be inferred using the algorithm W.
\\
\textbf{Significant Limitation: }
Let-polymorphism is rank-1 polymorphism, that means that functions cannot take as arguments polymorphic functions.
}

\end{block}
\end{frame}

\begin{frame}
\frametitle{Hindley-Milner typing}
\framesubtitle{Examples}
\begin{block}
{ 
     \begin{columns}[t] % contents are top vertically aligned
     \begin{column}[T]{5cm} % each column can also be its own environment
          \begin{figure}[h!]
				 \begin{small}
				 \rowcolors{1}{gray}{gray}
				 \begin{tabular}{l}
				 \textcolor{black}{
			      $>$ ./jebus annot} \\
			      \textcolor{black}{let const = \textbackslash x. \textbackslash y. x in} \\ \relax
			      \textcolor{black}{[const 1 true, const false 42]} \\
			      \textcolor{black}{-----------------------------} \\
			      \textcolor{black}{let const : a1 -> a2 -> a1 =} \\
			      \textcolor{black}{\tab \textbackslash x. : a1. \textbackslash y. : a6 . x}  \\
			      \textcolor{black}{in} \\ \relax
			      \textcolor{black}{\tab [const 1 true, const false 42]}
			      \end{tabular}	
				 \end{small}
			  \caption{Here \textit{const} has type $\forall a. \forall b. (a \rightarrow b \rightarrow a)$}
		 \end{figure}
     \end{column}
     \begin{column}[T]{5cm} % alternative top-align that's better for graphics
		 \begin{figure}[h!]
				\begin{small}
				\rowcolors{1}{gray}{gray}
			  	\begin{tabular}{l}
			      \textcolor{black}{$>$ ./jebus annot} \\
			      \textcolor{black}{let id = \textbackslash x.  x in}\\ \relax
			      \textcolor{black}{let f = \textbackslash g. [g 1, g true] in}\\
			      \textcolor{black}{\tab f id} \\
			      \textcolor{black}{Could not match type Nat with} \\
			      \textcolor{black}{type Bool}
				\end{tabular}	
			  \end{small}			  
			  \caption{g's type cannot be a polymorphic function!}
		 \end{figure}	          
     \end{column}
     \end{columns}
}

\end{block}
\end{frame}

%\frac{Gamma, x:\tau_1 \vdash e:\tau_2}{\Gamma \vdash \lambda x. e:\tau_1 \rightarrow \tau_2}var 
%\frac{}{\Gamma , x: \tau \vdash x:\tau }var  
 
\begin{frame}
\frametitle{Hindley-Milner typing}
\framesubtitle{Types}
\begin{block}{We will use $\tau$ for simple types, $\sigma$ for type schemes and $\alpha$ for type variables.}
\begin{align*}
\tau & := \tau_1\rightarrow \tau_2  &  \sigma  & := \forall  \alpha. \sigma_1\\
        & | \tau_1 \times \tau_2          &                      & | \;\tau \\
        & | Nat                                    & \\
        & | Bool                                  & \alpha & := \alpha _1 | \alpha _2| .... \\
        & | \alpha                                       & \\
\end{align*}
\end{block} 
\end{frame}  
 
\begin{frame}
\frametitle{Hindley-Milner typing}
\framesubtitle{Typing Rules}
\begin{block}{}
\begin{small}
\begin{align*}
& \frac{}{\Gamma , x: \sigma \vdash x:\sigma }var  
& \frac{\Gamma, x:\tau_1 \vdash e:\tau_2}{\Gamma \vdash \lambda x. e:\tau_1 \rightarrow \tau_2}\lambda \\[0.3cm]
& \frac{\Gamma \vdash e_1:\tau_1\rightarrow\tau_2 \;\; \Gamma \vdash e_2:\tau_1}{\Gamma \vdash e_1 \; e_2:\tau_2 }@ 
& \frac{\Gamma \vdash e_1:\sigma \;\;\Gamma, x:\sigma \vdash e_2:\tau}{\Gamma \vdash let \; [rec] \; x \; = e_1 \; in \; e_2:\tau }let \\[0.3cm]
& \frac{\Gamma \vdash e: \sigma \;\; \alpha \not \in FV(\Gamma)}{\Gamma \vdash e: \forall a. \sigma }gen 
& \frac{\Gamma \vdash e: \forall a. \sigma }{\Gamma \vdash e:\sigma [\alpha \rightarrow \tau ] }inst \\[0.3cm]
& \frac{\Gamma \vdash e : Bool \;\; \Gamma \vdash e_1:\tau \;\; \Gamma \vdash e_2:\tau}{\Gamma \vdash if \; e \; then \; e_2 \; else \;e_3 : \tau}ite
& \frac{\Gamma \vdash e_1:\tau_1 \;\; \Gamma \vdash e_2:\tau_2}{\Gamma \vdash [e_1, \; e_2]:\tau_1\times \tau_2  }pair \\[0.3cm]
\end{align*}
\end{small}
\end{block} 
\end{frame} 

\begin{frame}
\frametitle{Hindley-Milner typing}
\framesubtitle{Typing Rules (cont.)}
\begin{block}{}
\begin{small}
 \begin{gather*}
 \frac{\Gamma \vdash e_1 : Nat \;\; \Gamma \vdash e_2: Nat }{\Gamma \vdash e_1 \diamond e_2: Nat \;\;\; \diamond \in \lbrace +, -, *, /, **\rbrace}op \\[0.3cm]
 \frac{\Gamma \vdash e_1 : Nat \;\; \Gamma \vdash e_2: Nat }{\Gamma \vdash e_1 \diamond e_2: Bool \;\;\; \diamond \in \lbrace <, <=,==,>,>=\rbrace}rop \\[0.3cm]
 \frac{\Gamma \vdash e_1 : Bool \;\; \Gamma \vdash e_2: Bool }{\Gamma \vdash e_1 \diamond e_2: Bool \;\;\; \diamond \in \lbrace \&\&, || \rbrace }bop \\[0.3cm]
 \frac{\Gamma \vdash e : Bool }{\Gamma \vdash not \; e: Bool}not \\
\end{gather*}
\end{small}
\end{block} 
\end{frame} 

%

\begin{frame}
\frametitle{The Core Language}
\begin{block}{The internal representation is actually a pretty small language. Most of the language's expressions are defined as syntactic sugar}
\begin{align*}
e & := e_1 \; e_2 	 \\
   & | \; \bs{\lambda} \; id \; \bs{ .} \; e \\
   & | \; \bs{Fix} \; e_1                                                                 
\end{align*}
\end{block}
\end{frame}

%

\begin{frame}
\frametitle{The Core Language}
\framesubtitle{Syntactic Sugar}
\begin{block}{}
\begin{itemize}
\item \textbf{Integers} The integers are represented internally with church encoding\\
$$n \equiv \lambda \;s.\; \lambda \; z. \; \underbrace{s(s ... (s }_\text{n times} z)..)$$
\item \textbf{Arithmetical Operations} $e_1 + e_2 \equiv (\lambda \; x. \; \lambda \; y.\; x \; succ \; y) e_1 \; e_2$\\
$e_1 - e_2 \equiv (\lambda \; x. \; \lambda \; y.\; y \; pred \; x) e_1 \; e_2$ \\
$e_1 * e_2 \equiv (\lambda \; x. \; \lambda \; y.\; \lambda \; z. \;  x \; y \; z) e_1 \; e_2$ \\
$e_1 ** e_2 \equiv (\lambda \; x. \; \lambda \; y.\;  y \; x ) e_1 \; e_2$ \\
\end{itemize}
\end{block}
\end{frame}

\begin{frame}
\frametitle{The Core Language}
\framesubtitle{Syntactic Sugar}
\begin{block}{}
\begin{itemize}
\item \textbf{Boolean Constants} \\
$true \equiv \lambda \; x. \; \lambda \; y.\;  x \;\;\;\;\;\;$ 
$false \equiv \lambda \; x. \; \lambda \; y.\;  y$ \\
\item \textbf{Pairs} 
$[e_1, \; e_2] \equiv \lambda \;x.\; x \; e_1 \; e_2$ \\
\item \textbf{Provided functions for pairs} \\
$fst \equiv \lambda \;x.\; x \; true$ with type $\forall \;a. \forall b. \; a \times b \rightarrow a$\\
$snd \equiv \lambda \;x.\; x \; false$ with type $\forall \;a. \forall b. \; a \times b \rightarrow b$\\
\item \textbf{Provided functions for Integers} \\
$succ \equiv \lambda \; x. \; \lambda \; s. \; \lambda \; z. \;s \; (n \; s) \; z $ with type $Nat \rightarrow Nat$\\
$iszero \equiv \lambda \; x.\; x \; (true \; false) \; true $ with type $Nat \rightarrow Bool$ \\
$pred \equiv \lambda \; x.\; snd \; (x \; next \; [0,0] )$ with type $Nat \rightarrow Nat$ \\
where $next \equiv \lambda \; x. \; [succ \; (fst\;x), \; (fst\;x)]$
\end{itemize}
\end{block}
\end{frame}

\begin{frame}
\frametitle{The Core Language}
\framesubtitle{Syntactic Sugar}
\begin{block}{}
\begin{itemize}
\item \textbf{Boolean Operators} \\
$not \equiv \lambda \; x. \; x\; false\; true$ \\
$e_1 \&\& e_2 \equiv (\lambda \; x. \; \lambda \; y.\;  x \; y \; false) \; e_1 \; e_2$ \\
$e_1 || e_2 \equiv (\lambda \; x. \; \lambda \; y.\;  x \; true \; y) \; e_1 \; e_2$ \\
\item \textbf{Relative Operators} \\
$e_1 \leq e_2 \equiv (\lambda \; x. \; \lambda \; y.\; iszero \;(n\; pred \; m)) \; e_1 \; e_2$ \\
$e_1 < e_2 \equiv (\lambda \; x. \; \lambda \; y.\; not \;(y\; leq \; x)) \; e_1 \; e_2$ \\
$e_1 == e_2 \equiv (\lambda \; x. \; \lambda \; y.\; (y\; leq \; x) \&\&(x\; leq \; y))\; e_1 \; e_2$ \\
$e_1 \geq e_2 == e_2 \leq e_1 $ \\
$e_1 > e_2 == e_2 < e_1 $ \\
\end{itemize}
\end{block}
\end{frame}

\begin{frame}
\frametitle{The Core Language}
\framesubtitle{Syntactic Sugar}
\begin{block}{}
\begin{itemize}
\item \textbf{Let Definitions} \\
$let \; x \; = \; e_1 \; in \; e_2 \equiv (\lambda \; x. \;e_2 )\; e_1$ \\
\item \textbf{Let rec is more tricky} 
$let\; rec \; x \; = \; e_1 \; in \; e_2 \equiv (\lambda \; x. \;e_2 )\; (\bs{Y} \; (\lambda \; x. \;e_1 ))$ \\
remember that $Y \equiv \lambda \;f. \; (\lambda\; x. \; f \; (x\; x)) \; (\lambda\; x. \; f\;(x\;x))$
Alternatively, we can add a new construct to simulate $Y$'s behavior: 
$let\; rec \; x \; = \; e_1 \; in \; e_2 \equiv (\lambda \; x. \;e_2 )\; (\bs{Fix} \; (\lambda \; x. \;e_1 ))$ \\
In both cases $e_1$ is allowed to refer to $x$. The difference is that, unlike $Y$, $\bs{Fix}$ can be typed with the following rule:
$$ \frac{\Gamma \vdash e:\tau \rightarrow \tau}{\Gamma \vdash Fix \;e:\tau }fix  $$
\end{itemize}
\end{block}
\end{frame}

\begin{frame}
\frametitle{The Core Language}
\framesubtitle{Evaluation Strategies}
\begin{block}{
Currently Jebus supports two different evaluation strategies: normal order and applicative order, with the former being a 
non-strict evaluation strategy and the later a strict one.
}
In general:
\begin{itemize}
\item \textbf{Normal Order} The leftmost outermost redex is always reduced first
\\
\item \textbf{Applicative Order} The leftmost innermost redex is always reduced first
\end{itemize}

Both strategies evaluate the body of an unapplied  function.

\end{block}
\end{frame}

\begin{frame}
\frametitle{Evaluation Strategies}
\framesubtitle{Normal Order}
\begin{block}{The normal order reduction will always produce a normal form, if one exists!}
\begin{gather*}
\frac{}{ (\lambda \;x.\;e_1)\;e_2\rightarrow e_1 [e_2/x]} \\[0.25cm]
\frac{e_1\;\rightarrow \;e_1'}{e_1 \; e_2 \rightarrow e_1' \; e_2} \\[0.25cm]
\frac{e\;\rightarrow\;e'}{v \; e \rightarrow v \; e'} \\[0.25cm]
\frac{e\;\rightarrow\;e'}{\lambda\;x.\;e\; \rightarrow \lambda \;x. \;e'} \\[0.25cm]
\end{gather*}

\end{block}
\end{frame}


\begin{frame}
\frametitle{Evaluation Strategies}
\framesubtitle{Applicative Order}
\begin{block}{Applicative order reduction is not normalizing!}
\begin{gather*}
\frac{}{ (\lambda \;x.\;v_1)\;v_2\rightarrow v_1 [v_2/x]} \\[0.3cm]
\frac{e_1\;\rightarrow \;e_1'}{e_1 \; e_2 \rightarrow e_1' \; e_2} \\[0.3cm]
\frac{e\;\rightarrow\;e'}{v \; e \rightarrow v \; e'} \\[0.3cm]
\frac{e\;\rightarrow\;e'}{\lambda\;x.\;e\; \rightarrow \lambda \;x. \;e'} \\[0.3cm]
\end{gather*}
\end{block}
\end{frame}

\begin{frame}
\frametitle{Evaluation Strategies}
\framesubtitle{Semantics for fix}
\begin{block}{We can think fix as function that takes a function and computes its fixed point.}
\begin{gather*}
\frac{}{ (fix \; \lambda \;x.\;e) \rightarrow e[fix \; \lambda \; x. e/x]} \\[0.3cm]
\frac{e\;\rightarrow\;e'}{fix \; e \rightarrow fix \; e'} \\[0.3cm]
\end{gather*}

Note that $e[fix \; \lambda \; x. e/x] \equiv_\beta (\lambda\; x. e) \; (fix \; \lambda \; x. e) \equiv fix \; \lambda \; x. e$ ,
just like $f \;(Y\; f) \equiv Y \; f$.
\end{block}
\end{frame}


\begin{frame}
\frametitle{Evaluation Strategies}
\framesubtitle{Fix: Example}
\begin{block}{}
\begin{tiny}
\begin{align*}
 & let \; rec \; fact \; = \; \lambda \; x. \; if \; iszero \; x \; then \; 1 \; else \; x * fact \; (x-1) \; in \; fact \; 3 \\
 \rightarrow & (\lambda \; fact. \;fact \; 3 )\; (\bs{fix} \; (\lambda \; fact. \lambda \; x. \; if \; iszero \; x \; then \; 1 \; else \; x * fact \; (x-1))) \\
 \rightarrow & (\bs{fix} \; (\lambda \; fact. \lambda \; x. \; if \; iszero \; x \; then \; 1 \; else \; x * fact \; (x-1))) \; 3\\
\rightarrow & (\lambda \; x. \; if \; iszero \; x \; then \; 1 \; else \; x * (\bs{fix} \; (\lambda \; fact. \lambda \; x. \; if \; iszero \; x \; then \; 1 \; else \; x * fact \; (x-1))) \; (x-1)) \; 3\\ 
\rightarrow & if \; iszero \; 3 \; then \; 1 \; else \; 3 * (\bs{fix} \; (\lambda \; fact. \lambda \; x. \; if \; iszero \; x \; then \; 1 \; else \; x * fact \; (x-1))) \; (3-1) \\
\rightarrow &  3 * (\bs{fix} \; (\lambda \; fact. \lambda \; x. \; if \; iszero \; x \; then \; 1 \; else \; x * fact \; (x-1))) \; 2 \\
\rightarrow &  3 * (\lambda \; x. \; if \; iszero \; x \; then \; 1 \; else \; x * (\bs{fix} \; (\lambda \; fact. \lambda \; x. \; if \; iszero \; x \; then \; 1 \; else \; x * fact \; (x-1))) \; (x-1)) \; 2 \\
\rightarrow & 3 * if \; iszero \; 2 \; then \; 1 \; else \; 2 * (\bs{fix} \; (\lambda \; fact. \lambda \; x. \; if \; iszero \; x \; then \; 1 \; else \; x * fact \; (x-1))) \; (2-3) \\
\rightarrow & 3 * 2 * (\bs{fix} \; (\lambda \; fact. \lambda \; x. \; if \; iszero \; x \; then \; 1 \; else \; x * fact \; (x-1))) \; 1 \\
\rightarrow & 3 * 2 *(\lambda \; x. \; if \; iszero \; x \; then \; 1 \; else \; x * (\bs{fix} \; (\lambda \; fact. \lambda \; x. \; if \; iszero \; x \; then \; 1 \; else \; x * fact \; (x-1))) \; (x-1)) \; 1 \\
\rightarrow & 3 * 2 * if \; iszero \; 1 \; then \; 1 \; else \; 1 * (\bs{fix} \; (\lambda \; fact. \lambda \; x. \; if \; iszero \; x \; then \; 1 \; else \; x * fact \; (x-1))) \; (1-1) \; \\
\rightarrow & 3 * 2 * 1 * (\bs{fix} \; (\lambda \; fact. \lambda \; x. \; if \; iszero \; x \; then \; 1 \; else \; x * fact \; (x-1))) \; 0 \; \\
\rightarrow & 3 * 2 * 1 * (\lambda \; x. \; if \; iszero \; x \; then \; 1 \; else \; x * (\bs{fix} \; (\lambda \; fact. \lambda \; x. \; if \; iszero \; x \; then \; 1 \; else \; x * fact \; (x-1))) \; (x-1)) \; 0 \; \\
\rightarrow & 3 * 2 * 1 * if \; iszero \; 0 \; then \; 1 \; else \; 0 * (\bs{fix} \; (\lambda \; fact. \lambda \; x. \; if \; iszero \; x \; then \; 1 \; else \; x * fact \; (x-1))) \; (0-1) \\
\rightarrow & 3 * 2 * 1 *  1  \\
\end{align*}
\end{tiny}
\end{block}
\end{frame}


\begin{frame}
\frametitle{Evaluation Strategies}
\framesubtitle{Normal Order vs. Applicative Order}
\begin{block}{Consider the following programs:
  \begin{columns}[t] % contents are top vertically aligned
     \begin{column}[T]{5cm} % each column can also be its own environment
          \begin{figure}[h!]
				 \begin{footnotesize}
				 \rowcolors{1}{gray}{gray}
				 \begin{tabular}{l}
				 \textcolor{black}{
			      $>$ cat ite.lam} \\
			      \textcolor{black}{let f = \textbackslash x.} \\ 
			      \textcolor{black}{\tab  if (iszero x) then x + 3} \\
				  \textcolor{black}{\tab  else x * 3} \\
			      \textcolor{black}{in} \\
			      \textcolor{black}{\tab f 0} \\
			      \end{tabular}	
				 \end{footnotesize}
			  \caption{ite.lam}
		 \end{figure}
     \end{column}
     \begin{column}[T]{5cm} % alternative top-align that's better for graphics
		 \begin{figure}[h!]
				\begin{footnotesize}
				\rowcolors{1}{gray}{gray}
			  	\begin{tabular}{l}
			  	 \textcolor{black}{
			      $>$ cat fact.lam} \\
			      \textcolor{black}{let rec fact = \textbackslash x. } \\ 
			      \textcolor{black}{\tab if (iszero x) then 1} \\ 
			      \textcolor{black}{\tab else x * fact (x-1)} \\
			      \textcolor{black}{in} \\
			      \textcolor{black}{\tab fact 4} \\
				\end{tabular}	
			  \end{footnotesize}			  
			  \caption{fact.lam}
		 \end{figure}	          
     \end{column}
     \end{columns}
}
\end{block}
\end{frame}

\begin{frame}
\frametitle{Evaluation Strategies}
\framesubtitle{Normal Order vs. Applicative Order}
Applicative order needs 4 more beta reductions.  
Applicative order is a strict reduction strategy so both the then and the else parts
will be evaluated.
\begin{block}{
  \begin{columns}[T] % contents are top vertically aligned
     \begin{column}[T]{6cm} % each column can also be its own environment
          \begin{figure}[h!]
				 \begin{footnotesize}
				 \rowcolors{1}{gray}{gray}
				 \begin{tabular}{l}
				 \textcolor{black}{
			      $>$ ./jebus eval -e=normal -t < ite.lam} \\
			      \textcolor{black}{(\textbackslash f . f (\textbackslash f . \textbackslash x . x)) $\ldots \ldots$ =>} \\ 
			      \textcolor{black}{$\ldots$ =>} \\
				  \textcolor{black}{$\ldots$} \\
			      \textcolor{black}{$\ldots$ =>} \\
			      \textcolor{black}{\textbackslash f . \textbackslash x . f (f (f x))} \\
			      \textcolor{black}{Performed 11 beta reductions.} \\
			      \end{tabular}	
				 \end{footnotesize}
			  \caption{Evaluate ite.lam with normal order strategy. Only 11 beta reductions needed.}
		 \end{figure}
     \end{column}
     \begin{column}[T]{6cm} % alternative top-align that's better for graphics
		 \begin{figure}[h!]
				\begin{footnotesize}
				\rowcolors{1}{gray}{gray}
				 \begin{tabular}{l}
				 \textcolor{black}{
			      $>$ ./jebus eval -e=applicative -t < ite.lam} \\
			      \textcolor{black}{(\textbackslash f . f (\textbackslash f . \textbackslash x . x)) $\ldots \ldots$ =>} \\ 
			      \textcolor{black}{$\ldots$ =>} \\
				  \textcolor{black}{$\ldots$} \\
			      \textcolor{black}{$\ldots$ =>} \\
			      \textcolor{black}{\textbackslash f . \textbackslash x . f (f (f x))} \\
			      \textcolor{black}{Performed 14 beta reductions.} \\
			      \end{tabular}	
			  \end{footnotesize}			  
			  \caption{Evaluate ite.lam with applicative order strategy. 15 beta reductions needed.}
		 \end{figure}	          
     \end{column}
     \end{columns}
}

\end{block}
\end{frame}


\begin{frame}
\frametitle{Evaluation Strategies}
\framesubtitle{Normal Order vs. Applicative Order}
\begin{block}{
          \begin{figure}[h!]
				 \begin{footnotesize}
				 \rowcolors{1}{gray}{gray}
				 \begin{tabular}{l}
				 \textcolor{black}{
			      $>$ ./jebus eval -e=normal -t < fact.lam} \\
			      \textcolor{black}{((\textbackslash . fac (\textbackslash f . \textbackslash x . f (f (f (f x))))) $\ldots \ldots$ =>} \\ 
			      \textcolor{black}{$\ldots$ =>} \\
				  \textcolor{black}{$\ldots$} \\
			      \textcolor{black}{$\ldots$ =>} \\
			      \textcolor{black}{\textbackslash z . \textbackslash x . z (z (z (z (z (z (z (z (z (z (z (z (z (z (z (z (z (z (z (z (z (z (z (z x)...)} \\
			      \textcolor{black}{Performed 9236 beta reductions.} \\
			      \end{tabular}	
				 \end{footnotesize}
			  \caption{Evaluate fact.lam with normal order strategy. The program terminates after 9236 reductions.}
		 \end{figure}    
}

\end{block}
\end{frame}

\begin{frame}
\frametitle{Evaluation Strategies}
\framesubtitle{Normal Order vs. Applicative Order}
\begin{block}{
		 \begin{figure}[h!]
				\begin{footnotesize}
				\rowcolors{1}{gray}{gray}
				 \begin{tabular}{l}
				 \textcolor{black}{
			      $>$ ./jebus eval -e=applicative -t < fact.lam} \\
			      \textcolor{black}{((\textbackslash . fac (\textbackslash f . \textbackslash x . f (f (f (f x))))) $\ldots \ldots$ =>} \\ 
			      \textcolor{black}{$\ldots$ =>} \\
				  \textcolor{black}{$\ldots$} \\
			      \textcolor{black}{$\ldots$} \\
			      \end{tabular}	
			  \end{footnotesize}			  
			  \caption{Evaluate fact.lam with applicative order strategy. The program does not terminate.}
		 \end{figure}	          
}
\end{block}
\end{frame}

\begin{frame}
\frametitle{Useful links}
\begin{block}
{
\begin{footnotesize}
\begin{itemize}
\item \href{http://www.math.ntua.gr/logic/lambda/notes/shmeiwseis-2011.pdf}{Notes} form NTUA's Applications of Logic in Computer Science course %
\item \href{http://homepage.cs.uiowa.edu/~slonnegr/plf/Book/Chapter5.pdf}{Chapter 5} from the book Syntax and Semantics of Programming Languages, Kenneth Slonneger, Barry L. Kurtz
\item \href{http://www.cs.uu.nl/wiki/pub/Cco/CourseSchedule/cco-09-typesystems-2x2.pdf}{Hindley-Milner Typing and Algorithm W} from Compiler Construction course notes, Utrech University %
\item \href{http://lambda.jimpryor.net/lambda_library/}{lambda library} from NYU Lambda Seminar %
\item \href{http://homes.cs.washington.edu/~djg/2011sp/lec11_6up.pdf}{Simply typed lambda calculus extensions} from Programming Languages course notes, University of Washington %
\end{itemize}
\end{footnotesize}
}

\end{block}
\end{frame}

\begin{frame}
\frametitle{The end!}
\begin{block}
{\begin{center}
{\large Demo}
\end{center}}
\begin{center}
 \href{https://github.com/zoep/jebus}{Fork here!}
 \end{center} 
\end{block}
\end{frame}
% End of slides
\end{document} 
